# 正向和反向传播

## 前向传播

输入：$a^{[l−1]}$

输出：$a^{[l]}$，cache($z^{[l]}$, $w^{[l]}$, $b^{[l]}$)

公式：

$$
\begin{aligned}
z^{[l]} & = w^{[l]} \cdot a^{[l−1]} + b^{[l]} \\
a^{[l]} & = g^{[l]}(z^{[l]})
\end{aligned}
$$

向量化：

$$
\begin{aligned}
Z^{[l]} & = W^{[l]} \cdot A^{[l−1]} + b^{[l]} \\
A^{[l]} & = g^{[l]}(Z^{[l]})
\end{aligned}
$$

## 反向传播

输入：$da^{[l]}$

输出：$da^{[l−1]}$，$dw^{[l]}$，$db^{[l]}$

公式：

$$
\begin{aligned}
dz^{[l]} & = da^{[l]} \ast g^{[l] \prime}(z^{[l]}) \\
dw^{[l]} & = dz^{[l]} \cdot a^{[l−1]} \\
db^{[l]} & = dz^{[l]} \\
da^{[l−1]} & = w^{[l]T} \cdot dz^{[l]} \\
\end{aligned}
$$

向量化：

$$
\begin{aligned}
dZ^{[l]} & = dA^{[l]} \ast g^{[l] \prime}(Z^{[l]}) \\
dW^{[l]} & = \frac{1}{m} dZ^{[l]} \cdot A^{[l−1]} \\
db^{[l]} & = \frac{1}{m} \text{np.sum}( dZ^{[l]} \text{, axis = 1, keepdims = True}) \\
dA^{[l−1]} & = W^{[l]T} \cdot dZ^{[l]} \\
\end{aligned}
$$
